lib/Lib.Buffer.fsti
@@ -904,37 +904,64 @@ val mapi:
       as_seq h1 o == Seq.mapi (spec_f h0) (as_seq h i))
 
 #set-options "--z3rlimit 50"
-(*
+inline_for_extraction noextract
+val map_blocks_multi:
+    #t:buftype
+  -> #a:Type0
+  -> h0: mem
+  -> len:size_t{v len > 0}
+  -> blocksize:size_t{v blocksize > 0 /\ v len % v blocksize == 0}
+  -> inp:lbuffer_t t a len
+  -> output:lbuffer a len
+  -> spec_f:(mem -> GTot (i:nat{i < v len / v blocksize} -> Seq.lseq a (v blocksize) -> Seq.lseq a (v blocksize)))
+  -> impl_f:(i:size_t{v i < v len / v blocksize} -> Stack unit
+      (requires fun h1 ->
+	(v i + 1) * v blocksize <= max_size_t /\
+        modifies (loc (gsub output 0ul (i *! blocksize))) h0 h1)
+      (ensures  fun h1 _ h2 ->
+	let iblock = gsub inp (i *! blocksize) blocksize in
+	let oblock = gsub output (i *! blocksize) blocksize in
+        let ob = spec_f h0 (v i) (as_seq h1 iblock) in
+        B.modifies (loc oblock) h1 h2 /\
+        as_seq h2 oblock == ob))
+  -> Stack unit
+    (requires fun h -> h0 == h /\ live h output /\ live h inp /\ eq_or_disjoint inp output)
+    (ensures  fun _ _ h1 -> modifies1 output h0 h1 /\
+	as_seq h1 output == Seq.map_blocks_multi (v blocksize) (length inp / v blocksize) (as_seq h0 inp) (spec_f h0))
+
+
+
 inline_for_extraction noextract
 val map_blocks:
     #t:buftype
   -> #a:Type0
-  -> #len:size_t
   -> h0: mem
+  -> len:size_t
   -> blocksize:size_t{v blocksize > 0}
-  -> inp:lbuffer_t t a len 
-  -> output:lbuffer a len{eq_or_disjoint inp output}
+  -> inp:lbuffer_t t a len
+  -> output:lbuffer a len
   -> spec_f:(mem -> GTot (i:nat{i < v len / v blocksize} -> Seq.lseq a (v blocksize) -> Seq.lseq a (v blocksize)))
-  -> spec_l:(mem -> GTot (i:nat{i <= v len / v blocksize} -> llen:size_nat{llen < v blocksize} -> Seq.lseq a llen -> Seq.lseq a llen))
+  -> spec_l:(mem -> GTot (i:nat{i == v len / v blocksize} -> llen:size_nat{llen < v blocksize} -> Seq.lseq a llen -> Seq.lseq a llen))
   -> impl_f:(i:size_t{v i < v len / v blocksize} -> Stack unit
-      (requires fun h1 ->	modifies1 (gsub output 0ul (i *. blocksize)) h0 h1)
-      (ensures  fun h1 _ h2 -> 
-	v i * v blocksize + v blocksize <= v len /\
-       (let block = gsub output (i *. blocksize) blocksize in
-	modifies1 block h1 h2 /\
-	as_seq h2 block == spec_f h0 (v i) (as_seq h1 block))))
+      (requires fun h1 ->
+        (v i + 1) * v blocksize <= max_size_t /\
+        modifies (loc (gsub output 0ul (i *! blocksize))) h0 h1)
+      (ensures  fun h1 _ h2 ->
+        let iblock = gsub inp (i *! blocksize) blocksize in
+        let oblock = gsub output (i *! blocksize) blocksize in
+        let ob = spec_f h0 (v i) (as_seq h1 iblock) in
+        B.modifies (loc oblock) h1 h2 /\
+        as_seq h2 oblock == ob))
   -> impl_l:(i:size_t{v i == v len / v blocksize} -> Stack unit
-      (requires fun h1 ->	
-	modifies1 (gsub output 0ul (i *. blocksize)) h0 h1)
-      (ensures  fun h1 _ h2 -> 
-	v i * v blocksize + (v len % v blocksize) == v len /\
-       (let block = gsub output (i *. blocksize) (len %. blocksize) in
-	modifies1 block h1 h2 /\
-	as_seq h2 block == spec_l h0 (v i) (v len % v blocksize) (as_seq h1 block))))
+      (requires fun h1 ->
+        modifies (loc (gsub output 0ul (i *! blocksize))) h0 h1)
+      (ensures  fun h1 _ h2 ->
+        let iblock = gsub inp (i *! blocksize) (len %. blocksize)  in
+        let oblock = gsub output (i *! blocksize) (len %. blocksize) in
+        let ob = spec_l h0 (v i) (v len % v blocksize) (as_seq h1 iblock) in
+        B.modifies (loc oblock) h1 h2 /\
+        as_seq h2 oblock == ob))
   -> Stack unit
-    (requires fun h -> h0 == h /\ live h output)
+    (requires fun h -> h0 == h /\ live h output /\ live h inp /\ eq_or_disjoint inp output)
     (ensures  fun _ _ h1 -> modifies1 output h0 h1 /\
-	as_seq h1 output == Seq.map_blocks (v blocksize) (as_seq h0 inp) (spec_f h0) (spec_l h0))
-	  
-*)
-  
+        (admit (); as_seq h1 output == Seq.map_blocks (v blocksize) (as_seq h0 inp) (spec_f h0) (spec_l h0)))
