code/poly1305/Hacl.Impl.Poly1305.fsti
@@ -15,9 +15,7 @@ module F32xN = Hacl.Impl.Poly1305.Field32xN
 
 #reset-options "--z3rlimit 50"
 
-// The absence of inline_for_extraction / noextract is totally intentional. This relies on the
-// unsupported KreMLin feature that whenever an indexed type cannot be expressed in Low*, it gets
-// erased as "any", i.e. void*. In this case, this becomes "buffer any", i.e. void **.
+inline_for_extraction
 type poly1305_ctx (s:field_spec) = lbuffer (limb s) (nlimb s +. precomplen s)
 
 noextract
@@ -27,7 +25,7 @@ val as_get_r: #s:field_spec -> h:mem -> ctx:poly1305_ctx s -> GTot (S.elem (widt
 noextract
 val state_inv_t: #s:field_spec -> h:mem -> ctx:poly1305_ctx s -> Type0
 
-inline_for_extraction noextract
+inline_for_extraction
 val poly1305_init:
     #s:field_spec
   -> ctx:poly1305_ctx s
@@ -40,7 +38,7 @@ val poly1305_init:
       state_inv_t #s h1 ctx /\
       (as_get_acc h1 ctx, as_get_r h1 ctx) == S.poly1305_init (as_seq h0 key))
 
-inline_for_extraction noextract
+inline_for_extraction
 val poly1305_update:
     #s:field_spec
   -> ctx:poly1305_ctx s
@@ -53,9 +51,10 @@ val poly1305_update:
     (ensures  fun h0 _ h1 ->
       modifies (loc ctx) h0 h1 /\
       state_inv_t #s h1 ctx /\
-      as_get_acc h1 ctx == S.poly #(width s) (as_seq h0 text) (as_get_acc h0 ctx) (as_get_r h0 ctx))
+      Lib.Sequence.index (as_get_acc h1 ctx) 0 ==
+      S.poly_update #(width s) (as_seq h0 text) (as_get_acc h0 ctx) (as_get_r h0 ctx))
 
-inline_for_extraction noextract
+inline_for_extraction
 val poly1305_finish:
     #s:field_spec
   -> tag:lbuffer uint8 16ul
@@ -68,9 +67,9 @@ val poly1305_finish:
       state_inv_t #s h ctx)
     (ensures  fun h0 _ h1 ->
       modifies (loc tag |+| loc ctx) h0 h1 /\
-      as_seq h1 tag == S.finish #(width s) (as_seq h0 key) (as_get_acc h0 ctx))
+      as_seq h1 tag == S.finish (as_seq h0 key) (Lib.Sequence.index (as_get_acc h0 ctx) 0))
 
-inline_for_extraction noextract
+inline_for_extraction
 val poly1305_mac:
     #s:field_spec
   -> tag:lbuffer uint8 16ul
